borrow + live -> valid

src/resource_proofs.v
@@ -12,22 +12,89 @@ Require Import Burrow.rollup.
 Require Import Burrow.indexing.
 Require Import Burrow.locations.
 
-Definition live
-    {M} `{!EqDecision M, !Countable M, !TPCM M}
-    {RI} `{!EqDecision RI, !Countable RI}
-    (loc: Loc RI) (m: M) :=
-      StateCon empty_lifetime (build loc (CellCon m empty)).
+Require Import coqtricks.Deex.
+
+Instance loc_eqdec RI `{!EqDecision RI} `{!Countable RI} : EqDecision (Loc RI). Admitted.
+Instance loc_countable RI `{!EqDecision RI} `{!Countable RI} : Countable (Loc RI). Admitted.
+
+Definition lmap M `{!EqDecision M} `{!Countable M} `{!TPCM M}
+                RI `{!EqDecision RI, !Countable RI}
+  := gmap (Loc RI) (Cell M).
+Inductive State M `{!EqDecision M} `{!Countable M} `{!TPCM M}
+                RI `{!EqDecision RI, !Countable RI} :=
+  | StateCon : Lifetime -> lmap M RI -> State M RI
+.
+Arguments StateCon {M}%type_scope {EqDecision0 Countable0 TPCM0}
+    {RI}%type_scope {EqDecision1 Countable1} _ _.
     
-Definition reserved
-    {M} `{!EqDecision M, !Countable M, !TPCM M}
-    {RI} `{!EqDecision RI, !Countable RI}
-    (lt: Lifetime) (loc: Loc RI) (m:M) :=
-      StateCon empty_lifetime (build loc (CellCon unit {[ (lt,m) ]} )).
+Context {M} `{!EqDecision M} `{!Countable M} `{!TPCM M}.
+Context {RI} `{!EqDecision RI, !Countable RI}.
     
-Definition active
-    {M} `{!EqDecision M, !Countable M, !TPCM M}
-    (lt: Lifetime) : State M :=
-      StateCon lt BranchNil.
+Definition lmap_lookup (m : gmap (Loc RI) (Cell M)) (l : Loc RI) :=
+  match m !! l with None => triv_cell | Some c => c end.
+
+Definition lmaps_equiv (m1 m2 : gmap (Loc RI) (Cell M)) :=
+  ∀ l , lmap_lookup m1 l ≡ lmap_lookup m2 l.
+
+Global Instance state_equiv
+    : Equiv (State M RI) := λ x y ,
+  match x, y with
+  | StateCon lt1 m1, StateCon lt2 m2 =>
+      (lt1 = lt2 /\ lmaps_equiv m1 m2)
+  end.
+  
+Definition cell_op_opt (c1 c2 : option (Cell M)) := match c1, c2 with
+  | None, None => None
+  | Some c, None => Some c
+  | None, Some c' => Some c'
+  | Some c, Some c' => Some (c ⋅ c')
+end.
+
+Instance lmap_op : Op (lmap M RI) := λ x y ,
+    merge cell_op_opt x y.
+
+Instance state_op : Op (State M RI) := λ x y ,
+      match x, y with
+  | StateCon active1 lmap1, StateCon active2 lmap2 =>
+      StateCon (multiset_add active1 active2) (lmap1 ⋅ lmap2)
+  end.
+
+
+Definition live (loc: Loc RI) (m: M) :=
+      (*StateCon empty_lifetime (build loc (CellCon m empty)).*)
+      StateCon empty_lifetime {[ loc := CellCon m empty ]}.
+    
+Definition reserved (lt: Lifetime) (loc: Loc RI) (m:M) :=
+      StateCon empty_lifetime {[ loc := CellCon unit {[ (lt,m) ]} ]}.
+    
+Definition active (lt: Lifetime) : State M RI :=
+      StateCon lt ∅.
+
+Definition state_unit : State M RI := StateCon empty_lifetime ∅.
+
+Definition as_tree (l : lmap M RI) : Branch M :=
+  map_fold (λ k cell b , b ⋅ build k cell) BranchNil l.
+  
+Definition lmap_is_borrow (lt: Lifetime) (loc: Loc RI) (m: M) (l : lmap M RI) :=
+  forall pl , pl ∈ pls_of_loc loc ->
+    ∀ y , node_view (refinement_of_index M RI) (node_of_pl (as_tree l) pl) lt y -> tpcm_le m y.
+
+Definition is_borrow (lt: Lifetime) (loc: Loc RI) (m: M) (state: State M RI) :=
+    match state with
+    | StateCon _ l => lmap_is_borrow lt loc m l
+    end.
+  
+Definition state_inv (state: State M RI) : Prop :=
+  match state with
+  | StateCon active l =>
+       multiset_no_dupes active /\
+       branch_all_total_in_refinement_domain (refinement_of_index M RI) (as_tree l) active 0
+  end.
+
+Instance state_valid : Valid (State M RI) :=
+  λ v , ∃ p , state_inv (v ⋅ p).
+  
+Lemma as_tree_dot (a b: lmap M RI) : (as_tree a) ⋅ (as_tree b) ≡ as_tree (a ⋅ b). Admitted.
 
 (****************************************************************)
 (****************************************************************)
@@ -35,7 +102,7 @@ Definition active
 (****************************************************************)
 (* live(gamma, m) dot live(gamma, n) equiv live(gamma, m dot n) *)
 
-Lemma live_dot_live
+(*Lemma live_dot_live
     {M} `{!EqDecision M, !Countable M, !TPCM M}
     {RI} `{!EqDecision RI, !Countable RI}
     (gamma: Loc RI) (m1 m2: M)
@@ -52,4 +119,185 @@ Proof.
       + repeat (rewrite build_rest_triv); trivial.
           unfold triv_cell, "≡", cell_equiv, "⋅", cell_op. split.
           * apply unit_dot. * set_solver.
+Qed.
+*)
+
+Lemma lmaps_equiv_of_eq (a1 a2 : lmap M RI) (e: a1 = a2) : (lmaps_equiv a1 a2).
+Proof.  rewrite e. unfold lmaps_equiv. intro. apply cell_equiv_refl. Qed.
+
+Lemma live_dot_live
+    (gamma: Loc RI) (m1 m2: M)
+    : live gamma m1 ⋅ live gamma m2 ≡ live gamma (dot m1 m2).
+Proof.
+  unfold "≡", state_equiv, live. unfold "⋅", state_op. split.
+  - apply empty_add_empty_eq_empty.
+  - unfold lmaps_equiv. intro. unfold lmap_lookup. unfold "⋅", lmap_op.
+    rewrite lookup_merge. unfold diag_None.
+    assert (Decision (gamma = l)) by solve_decision. destruct H.
+    + rewrite e. repeat (rewrite lookup_singleton). unfold cell_op_opt.
+      unfold "≡", cell_equiv, "⋅", cell_op. split; trivial. set_solver.
+    + repeat (rewrite lookup_singleton_ne); trivial.
+Qed.
+
+(****************************************************************)
+(****************************************************************)
+(****************************************************************)
+(****************************************************************)
+(* live(gamma, unit) = unit *)
+
+Lemma live_unit (gamma : Loc RI) : live gamma unit ≡ state_unit.
+Proof.
+  unfold "≡", state_equiv, live, state_unit. split; trivial.
+  unfold lmaps_equiv. intro. unfold "≡". 
+  unfold lmap_lookup.
+  assert (Decision (gamma = l)) by solve_decision. destruct H.
+  - rewrite e. rewrite lookup_singleton. rewrite lookup_empty. unfold triv_cell.
+    apply cell_equiv_refl.
+  - rewrite lookup_singleton_ne; trivial. rewrite lookup_empty. unfold triv_cell.
+    apply cell_equiv_refl.
+Qed.
+    
+(****************************************************************)
+(****************************************************************)
+(****************************************************************)
+(****************************************************************)
+(* live(gamma, m) . borrow(kappa, gamma, k) --> valid (a . b) *)
+
+Instance state_equiv_symm : Symmetric state_equiv. Admitted.
+
+Instance branch_all_total_in_refinement_domain_proper roi :
+    Proper ((≡) ==> (=) ==> (=) ==> impl) (branch_all_total_in_refinement_domain roi).
+    Admitted.
+
+Instance branch_op_proper_left :
+    Proper ((≡) ==> (=) ==> (≡)) branch_op. Admitted.
+    
+Instance branch_op_proper_right b :
+    Proper ((≡) ==> (≡)) (branch_op b). Admitted.
+    
+Instance node_op_proper_left :
+    Proper ((≡) ==> (=) ==> (≡)) node_op. Admitted.
+    
+Instance node_op_proper_right n :
+    Proper ((≡) ==> (≡)) (node_op n). Admitted.
+    
+Instance cell_op_proper_left :
+    Proper ((≡) ==> (=) ==> (≡)) cell_op. Admitted.
+    
+Instance cell_op_proper_right n :
+    Proper ((≡) ==> (≡)) (cell_op n). Admitted.
+
+
+Instance node_view_proper roi :
+    Proper ((≡) ==> (=) ==> (=) ==> impl) (node_view roi). Admitted.
+    
+Instance node_live_proper :
+    Proper ((≡) ==> (=)) node_live. Admitted.
+    
+Instance cell_live_proper :
+    Proper ((≡) ==> (=)) cell_live. Admitted.
+    
+Lemma as_tree_singleton (loc: Loc RI) (cell: Cell M)
+  : as_tree {[loc := cell]} ≡ build loc cell. Admitted.
+
+Lemma forall_equiv_branch_all_total_in_refinement_domain roi branch lt idx
+  : branch_all_total_in_refinement_domain roi branch lt idx
+    <-> forall pl, node_all_total_in_refinement_domain roi (node_of_pl branch pl) lt (plend pl). Admitted.
+
+Definition any_pl_of_loc (loc: Loc RI) : PathLoc. Admitted.
+
+Lemma any_pl_of_loc_is_of_loc (loc: Loc RI)
+  : any_pl_of_loc loc ∈ pls_of_loc loc. Admitted.
+
+Lemma multiset_add_chain_included (a b c d : Lifetime) :
+  lifetime_included (multiset_add (multiset_add (multiset_add a b) c) d) a. Admitted.
+  
+Lemma in_refinement_domain_of_natird roi (node: Node M) (lifetime: Lifetime) (idx: nat)
+  (natird : node_all_total_in_refinement_domain roi node lifetime idx)
+      : in_refinement_domain roi idx (node_total roi node lifetime). Admitted.
+
+Lemma exists_some_of_match {A} (t: option A) (is_some : match t with | Some _ => True | None => False end)
+  : exists x , t = Some x. Admitted.
+
+(*node_view roi (a ⋅ b) k -> node_view roi a k
+            (node_of_pl (build gamma (CellCon m ∅) ⋅ as_tree l2 ⋅ as_tree l0)
+               (any_pl_of_loc gamma)) kappa
+            (node_total_minus_live (refinement_of_index M RI)
+               (node_of_pl (build gamma (CellCon m ∅) ⋅ as_tree l2 ⋅ as_tree l0)
+                  (any_pl_of_loc gamma))
+               (multiset_add (multiset_add (multiset_add kappa empty_lifetime) l1) l))*)
+
+Lemma node_view_le roi a b lt y : node_view roi (a ⋅ b) lt y -> node_view roi a lt y.
+Admitted.
+
+Lemma node_view_strip roi a b c loc kappa x :
+  node_view roi (node_of_pl (a ⋅ b ⋅ c) loc) kappa x ->
+  node_view roi (node_of_pl b loc) kappa x.
+Proof.  
+  intro.
+  setoid_rewrite <- forall_node_op in H.
+  assert (node_view roi (node_of_pl (a ⋅ b) loc) kappa x).
+  - apply node_view_le with (b := node_of_pl c loc). trivial.
+  - setoid_rewrite <- forall_node_op in H0.
+    setoid_rewrite node_op_comm in H0.
+    apply node_view_le with (b := node_of_pl a loc). trivial.
+Qed.
+
+Lemma node_node_cell_cell b pl : node_live (node_of_pl b pl) = cell_live (cell_of_pl b pl).
+Admitted.
+
+Lemma tpcm_le_m_node_live_with_m m gamma e b c
+    : tpcm_le m
+      (node_live (node_of_pl (build gamma (CellCon m e) ⋅ b ⋅ c) (any_pl_of_loc gamma))).
+Proof.
+  rewrite node_node_cell_cell.
+  setoid_rewrite <- forall_cell_op.
+  setoid_rewrite <- forall_cell_op.
+  setoid_rewrite build_spec.
+  - destruct (cell_of_pl b (any_pl_of_loc gamma)).
+    destruct (cell_of_pl c (any_pl_of_loc gamma)).
+    unfold cell_live. unfold "⋅", cell_op.
+    unfold tpcm_le. exists (dot m0 m1). apply tpcm_assoc.
+  - apply any_pl_of_loc_is_of_loc.
+Qed.
+
+Lemma live_and_borrow_implies_valid (gamma: Loc RI) (kappa: Lifetime) (m k: M) (b: State M RI)
+    (isb: is_borrow kappa gamma k b)
+    (isv: ✓(active kappa ⋅ live gamma m ⋅ b))
+    : m_valid (dot m k).
+Proof.
+  unfold "✓", state_valid in isv. deex. destruct p.
+  unfold state_inv in isv. unfold live in isv. destruct b. unfold "⋅" in isv.
+  unfold state_op in isv. destruct isv. clear H. rename H0 into isv.
+  unfold is_borrow, lmap_is_borrow in isb.
+  setoid_rewrite <- as_tree_dot in isv.
+  setoid_rewrite <- as_tree_dot in isv.
+  setoid_rewrite <- as_tree_dot in isv.
+  setoid_rewrite as_tree_singleton in isv.
+  generalize isv. clear isv. rewrite forall_equiv_branch_all_total_in_refinement_domain. intro isv.
+  
+  rename isb into isb'. have isb := isb' (any_pl_of_loc gamma) (any_pl_of_loc_is_of_loc gamma). clear isb'.
+  rename isv into isv'. have isv := isv' (any_pl_of_loc gamma). clear isv'.
+  have nvlt := node_view_le_total_minus_live _ _ _ _ _ _ isv.
+  have nvlt' := nvlt kappa (multiset_add_chain_included _ _ _ _). clear nvlt.
+  unfold view_sat in nvlt'.
+  
+  have nvlt'' := node_view_strip _ _ _ _ _ _ _ nvlt'.
+  have ineq := isb _ nvlt''.
+  
+  have ird := in_refinement_domain_of_natird _ _ _ _ isv.
+  unfold in_refinement_domain in ird.
+  rename ird into ird'. have ird := exists_some_of_match _ ird'. clear ird'. deex.
+  have elem_is_val := rel_valid_left _ _ _ _ _ ird.
+  clear ird.
+
+  assert (tpcm_le m (node_live 
+              (node_of_pl (build gamma (CellCon m ∅) ⋅ as_tree l2 ⋅ as_tree l0)
+                 (any_pl_of_loc gamma)))) by apply tpcm_le_m_node_live_with_m.
+  have summed_ineqs := le_add2 _ _ _ _ H ineq.
+  rewrite node_live_plus_node_total_minus_live in summed_ineqs.
+  unfold tpcm_le in summed_ineqs. deex.
+  rewrite <- summed_ineqs in elem_is_val.
+  have res := valid_monotonic _ _ elem_is_val.
+  trivial.
 Qed.
